theories/lang/pagetable_extra.v
@@ -187,6 +187,209 @@ Proof.
   { set_solver + H. }
 Qed.
 
+Lemma u_grnt_acc_acc σ ps v sacc:
+  set_Forall (λ p, is_Some ((get_page_table σ) !! p)) ps ->
+  get_access_gmap σ !! v = Some (to_dfrac_agree (DfracOwn 1) sacc) ->
+  get_access_gmap (update_page_table_global grant_access σ v ps)
+  =  <[v := to_dfrac_agree (DfracOwn 1) (ps ∪ sacc)]>(get_access_gmap σ).
+Proof.
+  rewrite /grant_access /update_page_table_global /=.
+  repeat destruct σ as [σ ?].
+  simpl.
+  intros Hforall Hlk.
+  apply map_eq.
+  intro.
+  destruct (decide (i = v)).
+  { subst.
+    rewrite lookup_insert.
+    revert Hforall Hlk.
+    generalize p.
+    generalize sacc.
+    induction ps as [|p' ps] using set_ind_L.
+    intros ? ? Hlk.
+    rewrite !set_fold_empty //.
+    rewrite union_empty_l_L //.
+    intros ? ?  Hlk.
+    rewrite !set_fold_disj_union_strong /=.
+    rewrite !set_fold_singleton.
+    destruct (p0 !! p') eqn: Hlk_p'.
+    2:{
+      specialize (Hlk p'). feed specialize Hlk.
+      set_solver.
+      simpl in Hlk.
+      rewrite Hlk_p' in Hlk.
+      inversion Hlk. done.
+    }
+    intro Hlookup.
+    rewrite (IHps ({[p']} ∪ sacc0)).
+    assert (ps ∪ ({[p']} ∪ sacc0) = {[p']} ∪ ps ∪ sacc0) as ->.
+    set_solver +.
+    done.
+    rewrite /get_access_gmap.
+    destruct p1.
+    intros p2 Hin_p2.
+    destruct (decide (p2 = p')).
+    { subst p2. rewrite lookup_insert. done. }
+    { rewrite lookup_insert_ne //. apply Hlk. set_solver + Hin_p2. }
+    rewrite /get_access_gmap /=.
+    rewrite fmap_insert /=.
+    destruct p1.
+    simpl.
+    rewrite -elem_of_list_to_map.
+    2:{
+      rewrite -list_fmap_compose.
+      simpl.
+      rewrite NoDup_fmap.
+      apply NoDup_list_of_vmids.
+    }
+    apply elem_of_list_In.
+    apply in_map_iff.
+    exists v.
+    split;auto.
+    2: apply in_list_of_vmids.
+    f_equal.
+    f_equal.
+    rewrite (map_filter_insert_True _ _ p').
+    2: { set_solver. }
+    rewrite dom_insert_L.
+    f_equal.
+    rewrite /get_access_gmap in Hlookup.
+    rewrite -elem_of_list_to_map in Hlookup.
+    2:{
+      rewrite -list_fmap_compose.
+      simpl.
+      rewrite NoDup_fmap.
+      apply NoDup_list_of_vmids.
+    }
+    apply elem_of_list_In in Hlookup.
+    apply in_map_iff in Hlookup.
+    destruct Hlookup as [? [Heq _]].
+    inversion Heq.
+    done.
+    2: set_solver + H.
+    {
+      intros.
+      destruct (b' !! x2) as [p2|] eqn: Hlookup2, (b' !! x1) as [p1|] eqn:Hlookup1;
+        rewrite ?lookup_insert_ne ?Hlookup1 ?Hlookup2 //;last eauto.
+      rewrite insert_commute //.
+    }
+  }
+  { rewrite lookup_insert_ne //.
+    destruct (get_access_gmap (σ, t0, p, v0, m, t) !! i) eqn: Hlookup.
+    {
+    revert Hforall Hlookup.
+    generalize p.
+    generalize sacc.
+    induction ps as [|p' ps] using set_ind_L.
+    intros ? ? Hforall.
+    rewrite !set_fold_empty //.
+    intros ? ?  Hforall Hlookup.
+    rewrite !set_fold_disj_union_strong /=.
+    rewrite !set_fold_singleton.
+    destruct (p0 !! p') eqn: Hlk_p'.
+    2:{
+      specialize (Hforall p'). feed specialize Hforall.
+      set_solver.
+      simpl in Hforall.
+      rewrite Hlk_p' in Hforall.
+      inversion Hforall. done.
+    }
+    rewrite (IHps ({[p']} ∪ sacc0)) //.
+    destruct p1.
+    intros p2 Hin_p2.
+    destruct (decide (p2 = p')).
+    { subst p2. rewrite lookup_insert. done. }
+    { rewrite lookup_insert_ne //. apply Hforall. set_solver + Hin_p2. }
+    rewrite /get_access_gmap /=.
+    rewrite fmap_insert /=.
+    destruct p1.
+    simpl.
+    rewrite -elem_of_list_to_map.
+    2:{
+      rewrite -list_fmap_compose.
+      simpl.
+      rewrite NoDup_fmap.
+      apply NoDup_list_of_vmids.
+    }
+    apply elem_of_list_In.
+    apply in_map_iff.
+    exists i.
+    split;auto.
+    2: apply in_list_of_vmids.
+    f_equal.
+    rewrite /get_access_gmap in Hlookup.
+    rewrite -elem_of_list_to_map in Hlookup.
+    2:{
+      rewrite -list_fmap_compose.
+      simpl.
+      rewrite NoDup_fmap.
+      apply NoDup_list_of_vmids.
+    }
+    apply elem_of_list_In in Hlookup.
+    apply in_map_iff in Hlookup.
+    destruct Hlookup as [? [Heq _]].
+    inversion Heq.
+    subst x.
+    f_equal.
+    destruct (decide (i ∈ g)).
+    rewrite (map_filter_insert_True _ _ p').
+    2: { set_solver + e. }
+    rewrite dom_insert_L.
+    assert (p' ∈ dom (gset PID) (filter (λ kv : PID * gset VMID, i ∈ kv.2) ((λ p2 : option VMID * bool * gset VMID, p2.2) <$> p0))).
+    {
+      rewrite elem_of_dom.
+      exists g.
+      rewrite map_filter_lookup_Some.
+      split;auto.
+      rewrite lookup_fmap_Some.
+      exists (p1,g).
+      split;done.
+    }
+    set_solver + H0.
+    rewrite (map_filter_insert_False _ _ p').
+    2: { set_solver + n0 n. }
+    rewrite map_filter_delete.
+    rewrite dom_delete_L.
+    assert (p' ∉ dom (gset PID) (filter (λ kv : PID * gset VMID, i ∈ kv.2) ((λ p2 : option VMID * bool * gset VMID, p2.2) <$> p0))).
+    {
+      rewrite elem_of_dom.
+      intro.
+      destruct H0.
+      rewrite map_filter_lookup_Some in H0.
+      destruct H0.
+      rewrite lookup_fmap_Some in H0.
+      destruct H0.
+      destruct H0.
+      subst x.
+      rewrite H3 in Hlk_p'.
+      inversion Hlk_p'.
+      subst x0.
+      set_solver + H1 n0.
+    }
+    set_solver + H0.
+    2: set_solver + H.
+    {
+      intros.
+      destruct (b' !! x2) as [p2|] eqn: Hlookup2, (b' !! x1) as [p1|] eqn:Hlookup1;
+        rewrite ?lookup_insert_ne ?Hlookup1 ?Hlookup2 //;last eauto.
+      rewrite insert_commute //.
+    }
+    }
+    rewrite /get_access_gmap in Hlookup.
+    rewrite -not_elem_of_list_to_map in Hlookup.
+    exfalso.
+    apply Hlookup.
+    rewrite -list_fmap_compose.
+    rewrite /fst.
+    cbn.
+    apply <- (elem_of_list_fmap (A:= fin vm_count) (B:= VMID)).
+    exists i.
+    split. done.
+    rewrite elem_of_list_In.
+    apply in_list_of_vmids.
+  }
+Qed.
+
 Lemma p_rvk_acc_current_vm σ i l:
   get_current_vm (update_page_table_global revoke_access σ i l) = get_current_vm σ.
 Proof. f_equal. Qed.
@@ -330,253 +533,40 @@ Proof.
   { set_solver + H. }
 Qed.
 
-Lemma u_grnt_acc_acc σ ps v sacc:
-  set_Forall (λ p, is_Some ((get_page_table σ) !! p)) ps ->
-  get_access_gmap σ !! v = Some (to_dfrac_agree (DfracOwn 1) sacc) ->
-  get_access_gmap (update_page_table_global grant_access σ v ps)
-  =  <[v := to_dfrac_agree (DfracOwn 1) (ps ∪ sacc)]>(get_access_gmap σ).
+Lemma u_flip_excl_excl σ ps v :
+ (get_excl_gmap (update_page_table_global flip_excl σ v ps)) = flip_excl_gmap (get_excl_gmap σ) ps.
 Proof.
-  rewrite /grant_access /update_page_table_global /=.
-  repeat destruct σ as [σ ?].
-  simpl.
-  intros Hforall Hlk.
-  apply map_eq.
-  intro.
-  destruct (decide (i = v)).
-  { subst.
-    rewrite lookup_insert.
-    revert Hforall Hlk.
-    generalize p.
-    generalize sacc.
-    induction ps as [|p' ps] using set_ind_L.
-    intros ? ? Hlk.
-    rewrite !set_fold_empty //.
-    rewrite union_empty_l_L //.
-    intros ? ?  Hlk.
-    rewrite !set_fold_disj_union_strong /=.
-    rewrite !set_fold_singleton.
-    destruct (p0 !! p') eqn: Hlk_p'.
-    2:{
-      specialize (Hlk p'). feed specialize Hlk.
-      set_solver.
-      simpl in Hlk.
-      rewrite Hlk_p' in Hlk.
-      inversion Hlk. done.
-    }
-    intro Hlookup.
-    rewrite (IHps ({[p']} ∪ sacc0)).
-    assert (ps ∪ ({[p']} ∪ sacc0) = {[p']} ∪ ps ∪ sacc0) as ->.
-    set_solver +.
-    done.
-    rewrite /get_access_gmap.
-    destruct p1.
-    intros p2 Hin_p2.
-    destruct (decide (p2 = p')).
-    { subst p2. rewrite lookup_insert. done. }
-    { rewrite lookup_insert_ne //. apply Hlk. set_solver + Hin_p2. }
-    rewrite /get_access_gmap /=.
-    rewrite fmap_insert /=.
-    destruct p1.
+  rewrite /get_excl_gmap.
+  rewrite /update_page_table_global /=.
+  rewrite /flip_excl_gmap /update_pgt_gmap /=.
+  generalize σ.1.1.1.2.
+  induction ps as [|p ps] using set_ind_L.
+  intros.
+  rewrite !set_fold_empty //.
+  intro pgt.
+  rewrite !set_fold_disj_union_strong /=.
+  rewrite !set_fold_singleton.
+  rewrite IHps.
+  rewrite lookup_fmap.
+  destruct (pgt!! p) eqn:Hlookup.
+  { rewrite Hlookup /=.
+    destruct p0.
     simpl.
-    rewrite -elem_of_list_to_map.
-    2:{
-      rewrite -list_fmap_compose.
-      simpl.
-      rewrite NoDup_fmap.
-      apply NoDup_list_of_vmids.
-    }
-    apply elem_of_list_In.
-    apply in_map_iff.
-    exists v.
-    split;auto.
-    2: apply in_list_of_vmids.
     f_equal.
-    f_equal.
-    rewrite (map_filter_insert_True _ _ p').
-    2: { set_solver. }
-    rewrite dom_insert_L.
-    f_equal.
-    rewrite /get_access_gmap in Hlookup.
-    rewrite -elem_of_list_to_map in Hlookup.
-    2:{
-      rewrite -list_fmap_compose.
-      simpl.
-      rewrite NoDup_fmap.
-      apply NoDup_list_of_vmids.
-    }
-    apply elem_of_list_In in Hlookup.
-    apply in_map_iff in Hlookup.
-    destruct Hlookup as [? [Heq _]].
-    inversion Heq.
+    destruct p0.
+    rewrite fmap_insert //=.
+  }
+  { rewrite Hlookup //=. }
+  2,4 : set_solver + H.
+  {
+    intros.
+    destruct (b' !! x2) as [p2|] eqn: Hlookup2, (b' !! x1) as [p1|] eqn:Hlookup1;
+      try destruct p1 as [q1 []]; try destruct p2 as [q2 []]; rewrite ?lookup_insert_ne ?Hlookup1 ?Hlookup2 //;last eauto.
+    apply insert_commute.
     done.
-    2: set_solver + H.
-    {
-      intros.
-      destruct (b' !! x2) as [p2|] eqn: Hlookup2, (b' !! x1) as [p1|] eqn:Hlookup1;
-        rewrite ?lookup_insert_ne ?Hlookup1 ?Hlookup2 //;last eauto.
-      rewrite insert_commute //.
-    }
   }
-  { rewrite lookup_insert_ne //.
-    destruct (get_access_gmap (σ, t0, p, v0, m, t) !! i) eqn: Hlookup.
-    {
-    revert Hforall Hlookup.
-    generalize p.
-    generalize sacc.
-    induction ps as [|p' ps] using set_ind_L.
-    intros ? ? Hforall.
-    rewrite !set_fold_empty //.
-    intros ? ?  Hforall Hlookup.
-    rewrite !set_fold_disj_union_strong /=.
-    rewrite !set_fold_singleton.
-    destruct (p0 !! p') eqn: Hlk_p'.
-    2:{
-      specialize (Hforall p'). feed specialize Hforall.
-      set_solver.
-      simpl in Hforall.
-      rewrite Hlk_p' in Hforall.
-      inversion Hforall. done.
-    }
-    rewrite (IHps ({[p']} ∪ sacc0)) //.
-    destruct p1.
-    intros p2 Hin_p2.
-    destruct (decide (p2 = p')).
-    { subst p2. rewrite lookup_insert. done. }
-    { rewrite lookup_insert_ne //. apply Hforall. set_solver + Hin_p2. }
-    rewrite /get_access_gmap /=.
-    rewrite fmap_insert /=.
-    destruct p1.
-    simpl.
-    rewrite -elem_of_list_to_map.
-    2:{
-      rewrite -list_fmap_compose.
-      simpl.
-      rewrite NoDup_fmap.
-      apply NoDup_list_of_vmids.
-    }
-    apply elem_of_list_In.
-    apply in_map_iff.
-    exists i.
-    split;auto.
-    2: apply in_list_of_vmids.
-    f_equal.
-    (* rewrite (map_filter_insert _ _ p'). *)
-    (* rewrite dom_insert_L. *)
-    (* f_equal. *)
-    rewrite /get_access_gmap in Hlookup.
-    rewrite -elem_of_list_to_map in Hlookup.
-    2:{
-      rewrite -list_fmap_compose.
-      simpl.
-      rewrite NoDup_fmap.
-      apply NoDup_list_of_vmids.
-    }
-    apply elem_of_list_In in Hlookup.
-    apply in_map_iff in Hlookup.
-    destruct Hlookup as [? [Heq _]].
-    inversion Heq.
-    subst x.
-    f_equal.
-    destruct (decide (i ∈ g)).
-    rewrite (map_filter_insert_True _ _ p').
-    2: { set_solver + e. }
-    rewrite dom_insert_L.
-    assert (p' ∈ dom (gset PID) (filter (λ kv : PID * gset VMID, i ∈ kv.2) ((λ p2 : option VMID * bool * gset VMID, p2.2) <$> p0))).
-    {
-      rewrite elem_of_dom.
-      exists g.
-      rewrite map_filter_lookup_Some.
-      split;auto.
-      rewrite lookup_fmap_Some.
-      exists (p1,g).
-      split;done.
-    }
-    set_solver + H0.
-    rewrite (map_filter_insert_False _ _ p').
-    2: { set_solver + n0 n. }
-    rewrite map_filter_delete.
-    rewrite dom_delete_L.
-    assert (p' ∉ dom (gset PID) (filter (λ kv : PID * gset VMID, i ∈ kv.2) ((λ p2 : option VMID * bool * gset VMID, p2.2) <$> p0))).
-    {
-      rewrite elem_of_dom.
-      intro.
-      destruct H0.
-      rewrite map_filter_lookup_Some in H0.
-      destruct H0.
-      rewrite lookup_fmap_Some in H0.
-      destruct H0.
-      destruct H0.
-      subst x.
-      rewrite H3 in Hlk_p'.
-      inversion Hlk_p'.
-      subst x0.
-      set_solver + H1 n0.
-    }
-    set_solver + H0.
-    2: set_solver + H.
-    {
-      intros.
-      destruct (b' !! x2) as [p2|] eqn: Hlookup2, (b' !! x1) as [p1|] eqn:Hlookup1;
-        rewrite ?lookup_insert_ne ?Hlookup1 ?Hlookup2 //;last eauto.
-      rewrite insert_commute //.
-    }
-    }
-    rewrite /get_access_gmap in Hlookup.
-    rewrite -not_elem_of_list_to_map in Hlookup.
-    exfalso.
-    apply Hlookup.
-    rewrite -list_fmap_compose.
-    rewrite /fst.
-    cbn.
-    set F := ((λ p0 : VMID * dfrac_agreeR (gsetO PID), let (x, _) := p0 in x)
-                ∘ (λ i0 : fin vm_count,
-                      (i0, to_frac_agree 1 (dom (gset PID) (filter (λ kv : PID * gset VMID, i0 ∈ kv.2) ((λ p0 : option VMID * bool * gset VMID, p0.2) <$> p)))))).
-    apply <- (elem_of_list_fmap (A:= fin vm_count) (B:= VMID)).
-    exists i.
-    split. done.
-    rewrite elem_of_list_In.
-    apply in_list_of_vmids.
-  }
+  apply upd_is_strong_assoc_comm.
 Qed.
-
-
-
-(*--- prove having mappings in gmap implies owership/access to pages in opsem ---*)
-
-(* TODO *)
-(* Lemma u_rvk_acc_acc σ ps v : *)
-(*   get_access_gmap (revoke_access_global σ v ps) = revoke_acc_gmap (get_access_gmap σ) v ps. *)
-(* Proof. *)
-(*   rewrite /get_access_gmap. *)
-(*   rewrite /revoke_access_global /update_page_table_global /=. *)
-(*   rewrite /revoke_acc_gmap /update_acc_gmap /=. *)
-(*   generalize  σ.1.1.1.2. *)
-(*   induction ps as [|p ps] using set_ind_L. *)
-(*   intros. *)
-(*   rewrite !set_fold_empty //. *)
-(*   intro pgt. *)
-(*   rewrite !set_fold_disj_union_strong /=. *)
-(*   rewrite !set_fold_singleton. *)
-(*   rewrite IHps. *)
-(*   rewrite lookup_fmap. *)
-(*   destruct (pgt!! p) eqn:Hlookup. *)
-(*   { rewrite Hlookup /=. *)
-(*     destruct p0. *)
-(*     simpl. *)
-(*     f_equal. *)
-(*     rewrite fmap_insert //=. *)
-(*   } *)
-(*   { rewrite Hlookup //=. } *)
-(*   2,4 : set_solver + H. *)
-(*   { *)
-(*     intros. *)
-(*     destruct (b' !! x2) as [p2|] eqn: Hlookup2, (b' !! x1) as [p1|] eqn:Hlookup1; *)
-(*       try destruct p1 as [q1 []]; try destruct p2 as [q2 []]; rewrite ?lookup_insert_ne ?Hlookup1 ?Hlookup2 //;last eauto. *)
-(*     apply insert_commute. *)
-(*     done. *)
-(*   } *)
-(*   apply upd_is_strong_assoc_comm. *)
-(* Qed. *)
 
 Lemma p_upd_pgt_pgt_not_elem {i:VMID} {perm : permission} pgt upd (sps: gset PID) (p:PID) :
   p ∉ sps ->
